Use unproven spec for incr service in MakePreparedRequest proof.
Need to weaken spatial context to the loop invariant for the
MakePreparedRequest proof, just like in the proof of MakeRequest.

Had to do a bit of work to turn a
`(readonly (ck ↦[ShortTermIncrClerk.S :: "req"] <struct literal>))`
into a bunch of readonly ptstos for all of the fields in the req struct,
to satisfy the read_request precondition of RemoteProcedureCall_spec.

src/program_proof/lockservice/incr_proxy_proof.v
@@ -38,8 +38,6 @@ Axiom is_incrserver : incrservice_names → loc → iProp Σ.
 Instance is_incrserver_pers γ incrserver : Persistent (is_incrserver γ incrserver).
 Admitted.
 
-Axiom own_incrclerk : incrservice_names → loc → loc → iProp Σ.
-
 Variable γ:incrservice_names.
 
 Context `{!kvserviceG Σ}.
@@ -48,8 +46,7 @@ Definition ProxyIncrServer_core_own (srv:loc) : iProp Σ :=
   ∃ (kck incrserver:loc),
   "Hkvserver" ∷ srv ↦[IncrProxyServer.S :: "incrserver"] #incrserver ∗
   "Hkck" ∷ srv ↦[IncrProxyServer.S :: "ick"] #kck ∗
-  "His_kvserver" ∷ is_incrserver γ incrserver ∗
-  "Hkck_own" ∷ own_incrclerk γ kck incrserver
+  "His_kvserver" ∷ is_incrserver γ incrserver
   (* This is using the non-crash-safe version of kvserver in kv_proof.v *)
 .
 
@@ -76,14 +73,102 @@ Proof.
   iFrame. done.
 Qed.
 
-Definition own_short_incr_clerk ck isrv (cid seq:u64) (args:RPCValC) : iProp Σ :=
+Definition own_short_incr_clerk (ck isrv:loc) (cid seq:u64) (args:RPCValC) : iProp Σ :=
   "cid" ∷ ck ↦[ShortTermIncrClerk.S :: "cid"] #cid ∗
   "seq" ∷ ck ↦[ShortTermIncrClerk.S :: "seq"] #seq ∗
   "incrserver" ∷ ck ↦[ShortTermIncrClerk.S :: "incrserver"] #isrv ∗
-  "req" ∷ ck ↦[ShortTermIncrClerk.S :: "req"] (#cid,
+  "req" ∷ (* ck ↦[ShortTermIncrClerk.S :: "req"] req_ptr ∗
+  "Hread_req" ∷ read_request req_ptr {| Req_CID:=cid; Req_Seq:=seq; Req_Args:=args|} ∗ *)
+
+
+  (readonly (ck ↦[ShortTermIncrClerk.S :: "req"] (#cid,
                                               (#(word.sub seq 1:u64),
-                                              (#args.1, (#args.2.1, #()), #())))
+                                              (#args.1, (#args.2.1, #()), #())))))
 .
+
+Variable c:nat. (* Old value of the ghost counter *)
+Definition IncrPreCond : RPCValC → iProp Σ := (λ a, a.1 fm[[γ.(incr_mapGN)]]↦ c)%I.
+Definition IncrPostCond : RPCValC → u64 → iProp Σ := (λ a r, a.1 fm[[γ.(incr_mapGN)]]↦ (c+1))%I.
+
+Context `{!rpcG Σ (@RPCReply u64)}.
+
+(* TODO: will want to use merged rpc_base+rpc_durable *)
+Definition own_prepared_short_incr_clerk ck isrv cid seq args : iProp Σ :=
+  own_short_incr_clerk ck isrv cid seq args ∗
+  ⌜(int.nat (word.sub seq 1%nat) > 0)%Z⌝ ∗
+  ∃ γPost, is_RPCRequest γ.(incr_rpcGN) γPost IncrPreCond IncrPostCond {| Req_CID:=cid; Req_Seq:=(word.sub seq 1:u64); Req_Args:=args |}
+.
+
+(* TODO: this should refer to a lemma in incr_proof.v *)
+
+Lemma IncrServer__Increment_is_rpcHandler (isrv:loc) :
+is_incrserver γ isrv -∗
+{{{
+     True
+}}}
+  IncrServer__Increment #isrv
+{{{ (f:goose_lang.val), RET f;
+        is_rpcHandler f γ.(incr_rpcGN) IncrPreCond IncrPostCond
+}}}.
+Admitted.
+
+Lemma wp_ShortTermIncrClerk__MakePreparedRequest ck isrv cid seq args :
+is_incrserver γ isrv -∗
+{{{
+     own_prepared_short_incr_clerk ck isrv cid seq args
+}}}
+    ShortTermIncrClerk__MakePreparedRequest #ck
+{{{
+     RET #(); True
+}}}
+.
+Proof.
+  iIntros "#Hs_inv" (Φ) "!# (Hown_ck & %Hseq_ineq & HreqInv) Hpost".
+  wp_lam.
+  wp_apply wp_ref_to; first eauto.
+  iIntros (errb) "Herrb".
+  wp_pures.
+  wp_apply (wp_allocStruct); first eauto.
+  iIntros (reply) "Hreply".
+  wp_pures.
+  iNamed "HreqInv".
+  iDestruct "HreqInv" as "#HreqInv".
+  iNamed "Hown_ck".
+  wp_forBreak.
+  wp_pures.
+
+  (* Transform the readonly struct field into a bunch of readonly ptsto for each field via fieldRef *)
+  iMod (readonly_load with "req") as (q) "req".
+  wp_apply (wp_struct_fieldRef_mapsto with "req"); first done.
+  iIntros (req) "[%Hacc_req Hreq]".
+  iDestruct (struct_fields_split with "Hreq") as "Hreq".
+  iNamed "Hreq".
+  iMod (readonly_alloc (req ↦[RPCRequest.S :: "CID"] #cid) q with "[CID]") as "#CID"; first eauto.
+  iMod (readonly_alloc (req ↦[RPCRequest.S :: "Seq"] #(word.sub seq 1:u64)) q with "[Seq]") as "#Seq"; first eauto.
+  iMod (readonly_alloc (req ↦[RPCRequest.S :: "Args"] (into_val.to_val args)) q with "[Args]") as "#Args"; first eauto.
+
+  wp_loadField.
+  wp_apply (IncrServer__Increment_is_rpcHandler with "Hs_inv").
+  iIntros (f) "#His_rpcHandler".
+  wp_apply (RemoteProcedureCall_spec with "His_rpcHandler [$HreqInv $CID $Seq $Args Hreply]").
+  {
+    Opaque struct.t.
+    simpl.
+    Transparent struct.t.
+    Print own_reply.
+    iDestruct (struct_fields_split with "Hreply") as "Hreply".
+    iNamed "Hreply".
+    instantiate (1:={| Rep_Stale:=_; Rep_Ret:=_|}).
+    by iFrame.
+  }
+  iIntros (e) "HrpcPost".
+  iDestruct "HrpcPost" as (reply') "[Hown_reply [%He|HrpcPost]]".
+  - rewrite He. wp_store. wp_load. wp_binop. wp_pures.
+    iLeft.
+    iFrame.
+    (* Need to weaken "loop invariant" before wp_forBreak *)
+    admit.
+Admitted.
 
 Lemma wp_DecodeShortTermIncrClerk cid seq args (isrv:loc) (content:Slice.t) data :
 {{{
@@ -171,6 +256,7 @@ Proof.
   iDestruct (Hacc_req with "Hreq") as "req".
   clear Hacc_req req.
 
+  iApply wp_fupd.
   wp_apply (wp_Dec__GetInt with "His_dec").
   iIntros "His_dec".
 
@@ -194,8 +280,9 @@ Proof.
   iDestruct (Hacc_req with "Hreq") as "req".
   clear Hacc_req req.
 
+  iMod (readonly_alloc_1 with "req") as "req".
   iApply "HΦ".
-  iFrame.
+  by iFrame.
 Qed.
 
 Lemma increment_proxy_core_indepotent (isrv:loc) (seq:u64) (args:RPCValC) :
